coq-minuska/theories/builtin/list_signature.v
@@ -59,26 +59,7 @@ Next Obligation.
 Qed.
 Fail Next Obligation.
 
-Program Definition list_signature : Signature := {|
+Definition list_signature : Signature := {|
     builtin_function_symbol := ListFunSymbol ;
     builtin_predicate_symbol := ListPredSymbol ;
-    bps_ar := fun p =>
-        match p with
-        | list_is => 1
-        end ;
-    bps_neg := fun p =>
-        match p with
-        | list_is => None
-        end ;
-    bps_neg_ar := _ ;
-    bps_neg__sym := _;
 |}.
-Next Obligation.
-    destruct p,p'; simpl in *; reflexivity.
-Qed.
-Next Obligation.
-    destruct p,p'; simpl in *; ltac1:(simplify_eq/=).
-Qed.
-Fail Next Obligation.
-
-
